Clean up HOL sources.  In particular, actions have at most one write.
Previously actions could have lists of writes stored in them, even
though the remainder were ignored.  This was done as a hacky solution
to a problem that the hierarchical DAGs solve much better.

Some bad solutions to the nested/hierarchical DAG problem also
deleted.

hol/actiongraphs/actionScript.sml
@@ -11,7 +11,7 @@ val _ = new_theory "action";
 val _ = IndDefLib.export_rule_induction "relation.TC_STRONG_INDUCT"
 val _ = Hol_datatype`
   action = <|
-    writes : 'rw list;
+    write : 'rw option;
     reads : 'rw list ;
     data : 'data;
     ident : 's_ident
@@ -21,12 +21,18 @@ val _ = Hol_datatype`
 `;
 
 val action_component_equality = theorem "action_component_equality"
+val optset_def = Define`
+  optset NONE = ∅ ∧
+  optset (SOME x) = {x}
+`;
+val _ = overload_on ("set", ``optset``)
+val _ = export_rewrites ["optset_def"]
 
 val touches_def = Define`
   touches a1 a2 ⇔
-     (∃w. MEM w a1.writes ∧ MEM w a2.writes) ∨
-     (∃w. MEM w a1.writes ∧ MEM w a2.reads) ∨
-     (∃w. MEM w a2.writes ∧ MEM w a1.reads)
+     ¬DISJOINT (set a1.reads) (set a2.write) ∨
+     ¬DISJOINT (set a2.reads) (set a1.write) ∨
+     ¬DISJOINT (set a1.write) (set a2.write)
 `;
 
 val _ = set_mapped_fixity {term_name = "touches", fixity = Infix(NONASSOC, 450),
@@ -46,13 +52,13 @@ val _ = export_rewrites ["touches_ignores_ident"]
 val touches_SYM = store_thm(
   "touches_SYM",
   ``touches a1 a2 ⇒ touches a2 a1``,
-  simp[touches_def] >> rpt strip_tac >> simp[] >> metis_tac[]);
+  simp[touches_def] >> rpt strip_tac >> simp[] >> metis_tac[DISJOINT_SYM]);
 
 (* redundant if HOL's github issue #173 is fixed *)
 val polydata_upd_def = Define`
   polydata_upd f a = <|
     reads := a.reads ;
-    writes := a.writes ;
+    write := a.write ;
     data := f a.data;
     ident := a.ident
   |>`
@@ -64,7 +70,7 @@ val polydata_upd_ident = store_thm(
 
 val polydata_upd_reads_writes = store_thm(
   "polydata_upd_reads_writes[simp]",
-  ``(polydata_upd f a).reads = a.reads ∧ (polydata_upd f a).writes = a.writes``,
+  ``(polydata_upd f a).reads = a.reads ∧ (polydata_upd f a).write = a.write``,
   simp[polydata_upd_def]);
 
 val polydata_upd_data = store_thm(
